@prefix foaf: <http://xmlns.com/foaf/0.1/> .
@prefix rdf: <http://www.w3.org/1999/02/22-rdf-syntax-ns#> .
@prefix rdfs: <http://www.w3.org/2000/01/rdf-schema#> .
@prefix dct: <http://purl.org/dc/terms/> .
@prefix dc: <http://purl.org/dc/elements/1.1/> .
@prefix owl: <http://www.w3.org/2002/07/owl#> .
@prefix xsd: <http://www.w3.org/2001/XMLSchema#> .
@prefix cc: <http://creativecommons.org/ns#> .

@prefix odil:	<http://schema.theodi.org/open-data-licensing#> .

############################################################################
# General description of the ontology
############################################################################

<http://schema.theodi.org/open-data-licensing#>
    a owl:Ontology;
    owl:versionInfo "0.1";
    rdfs:label "Open Data Rights Statement Schema";
    rdfs:comment "Provides an ontology for describing rights statements, e.g. licenses, copyright notices, attribution requirements, for Open Datasets.";
    dct:created "2013-05-31"^^xsd:date;
    dct:title "Open Data Rights Statement Schema"@en;
    foaf:maker <http://www.ldodds.com#me>.

<http://www.ldodds.com#me> a foaf:Person ;
	foaf:name "Leigh Dodds" .

############################################################################
# Classes
############################################################################

odil:RightsStatement
	a owl:Class;	
    rdfs:label "Rights Statement"@en;
    rdfs:comment """A description of the rights and terms of re-use for a dataset. A rights statement will include a reference to one or more licenses (covering the data and content domains), copyright notices, and attribution requirements."""@en;
	rdfs:subClassOf dct:RightsStatement.

odil:License
	a owl:Class;	
    rdfs:label "License"@en;
    rdfs:comment """A legal document that describes the legal terms for re-use of some information. A license might apply to either content or data. It might also be a waiver document that indicates that the owner waives all rights they may have over the information."""@en;
	rdfs:subClassOf dct:LicenseDocument;
	owl:equivalentClass cc:License.

############################################################################
# Object Properties
############################################################################

odil:dataLicense
	a owl:ObjectProperty;
	rdfs:label "data license"@en;
	rdfs:comment "Indicates which data license is applicable to the dataset(s) referencing a rights statement."@en;
	rdfs:subPropertyOf dct:license;
	rdfs:domain odil:RightsStatement;
	rdfs:range odil:License.
	
odil:contentLicense
	a owl:ObjectProperty;
	rdfs:label "content license"@en;
	rdfs:comment "Indicates which content license is applicable to the dataset(s) referencing a rights statement"@en;
	rdfs:subPropertyOf dct:license;
	rdfs:domain odil:RightsStatement;
	rdfs:range odil:License.

odil:rights
	a owl:ObjectProperty;
	rdfs:label "rights"@en;
	rdfs:comment "associates a rights statement with a dataset"@en;
	owl:equivalentProperty dct:rights;
	rdfs:range odil:RightsStatement.

############################################################################
# Datatype Properties
############################################################################

odil:copyrightNotice
	a owl:DatatypeProperty;
	rdfs:label "copyright notice"@en;
	rdfs:comment "The copyright notice associated with a rights statement. A notice must typically be preserved and displayed when acknowledging the source of some data"@en;    
	rdfs:range rdfs:Literal;
	rdfs:domain odil:RightsStatement.

odil:attributionName
	a owl:DatatypeProperty;
	rdfs:label "attribution name"@en;
	rdfs:comment "The name of the rights holder, to be used when attributing the publisher of a dataset"@en;    
	rdfs:range rdfs:Literal;
	rdfs:domain odil:RightsStatement.

odil:attributionURL
	a owl:DatatypeProperty;
	rdfs:label "attribution url"@en;
	rdfs:comment "The URL to be used when attributing a data source."@en;    
	rdfs:range rdfs:Literal;
	rdfs:domain odil:RightsStatement.
